test/Mutable/UnionFind.lean
@@ -1,0 +1,23 @@
+import Algorithm.Data.UnionFind
+
+abbrev Vector.WithDefault := Batteries793.Vector.WithDefault
+abbrev UF := UnionFind (Fin 10)
+  (Vector.WithDefault (Fin 10) 10 id)
+  (Vector.WithDefault Nat 10 (fun _ ↦ 1))
+
+#eval show IO Unit from do
+  let mut uf : UF := default
+  IO.println (uf.find 1)
+  uf := uf.union 1 2
+  uf := uf.union 3 4
+  uf := uf.union 2 4
+  IO.println ((Quot.unquot (Mutable.get uf)).val.parent[(1 : Fin 10)])
+
+#eval show IO Unit from do
+  let mut uf : UF := default
+  IO.println (uf.find 1)
+  uf := uf.union 1 2
+  uf := uf.union 3 4
+  uf := uf.union 2 4
+  IO.println (uf.find 1)
+  IO.println ((Quot.unquot (Mutable.get uf)).val.parent[(1 : Fin 10)])
