test/Mutable/thunk3.lean
@@ -1,0 +1,41 @@
+import Algorithm.Data.Mutable
+
+universe u
+
+def Thunk' (α : Type u) : Type u := Mutable (Unit → α)
+
+variable {α : Type u}
+
+def Thunk'.mk (fn : Unit → α) : Thunk' α := Mutable.mk fn
+
+protected def Thunk'.pure (a : α) : Thunk' α :=
+  .mk fun _ ↦ a
+
+protected def Thunk'.get (x : Thunk' α) : α :=
+  Mutable.getModify₂ x (fun f ↦ let a := f (); ⟨a, fun _ ↦ a⟩) (fun _ ↦ rfl)
+
+@[inline] protected def Thunk'.map (f : α → β) (x : Thunk' α) : Thunk' β :=
+  .mk fun _ => f x.get
+
+@[inline] protected def Thunk'.bind (x : Thunk' α) (f : α → Thunk' β) : Thunk' β :=
+  .mk fun _ => (f x.get).get
+
+def List.sum [OfNat α 0] [Add α] : List α → α :=
+  foldl (· + ·) 0
+
+#eval show IO Unit from do
+  let _ : OfNat (Thunk' Nat) 0 := ⟨.pure 0⟩
+  let _ : Inhabited (Thunk' Nat) := ⟨.pure 0⟩
+  let _ : Add (Thunk' Nat) := ⟨fun x y ↦ .mk fun _ ↦ x.get + y.get⟩
+  let mut l := [Thunk'.pure 1]
+  for _ in [0 : 32] do
+    l := l.sum :: l
+  IO.println l.head!.get
+#eval show IO Unit from do
+  let _ : OfNat (Thunk' Nat) 0 := ⟨.pure 0⟩
+  let _ : Inhabited (Thunk' Nat) := ⟨0⟩
+  let _ : Add (Thunk' Nat) := ⟨fun x y ↦ .mk fun _ ↦ x.get + y.get⟩
+  let mut l := [1]
+  for _ in [0 : 32] do
+    l := l.sum :: l
+  IO.println l.head!
